#+title: Przykladowyegzamin

* Zad 1
\begin{align*}
\Im \left(\frac{1+3i}{3-2i} + i^{3} + 5\right)
 &=\Im \left(\frac{1+3i}{3-2i} + \frac{i^{3}(3-2i)}{3-2i} + \frac{5(3-2i)}{3-2i}\right)\\
 &= \Im \left(\frac{1+3i + 3i^3 - 2 i^4 + 15 - 10i}{3-2i}\right)\\
 &= \Im \left(\frac{16 - 7i + 3i^{3} -2i^{4}}{3-2i}\right)\\
 &= \Im \left(\frac{14 - 10i}{3-2i}\right)\\
 &= \Im \left(\frac{14 - 10i}{3-2i} \cdot \frac{3+2i}{3+2i}\right)\\
 &= \Im \left(\frac{42 + 28i - 30i + 20}{9 + 4}\right)\\
 &= \Im \left(\frac{62 - 2i }{13}\right)\\
 &= \frac{-2}{13}
\end{align*}
* Zad 2
\begin{align*}
  \frac{ { (3 - 3i)}^{14} }
  { { (-1+i\sqrt{3}) }^{11} }
  &= \frac{z^{14}}{w^{11}}
\end{align*}
** $z$
$$\sin(\varphi_z) = \frac{-3}{3\sqrt{2}}
 = \frac{-1}{\sqrt{2}}
 = \frac{-\sqrt{2}}{2} \to \varphi_z = \frac{7}{4}\pi$$

\begin{align*}
  z^{14} &= {(3 - 3i)}^{14}\\
  &= {(3-3i)}^{14}\\
  &= {(3\sqrt{2})}^{14}(\cos 14 \varphi + i \sin 14 \varphi)\\
  &= {(3\sqrt{2})}^{14} \left(\cos \left(14 \cdot \frac{7}{4} \pi \right) + i \sin \left(14 \cdot \frac{7}{4} \pi \right) \right)\\
  &= {(3\sqrt{2})}^{14} \left( \cos \left ( \frac{49}{2} \pi \right) + i \sin \left(\frac{49}{2} \pi \right) \right)\\
  &= {(3\sqrt{2})}^{14} \left( \cos \left ( \frac{1}{2} \pi \right) + i \sin \left(\frac{1}{2} \pi \right) \right)\\
  &= {(3\sqrt{2})}^{14} ( 0 + i 1 )\\
  &= {(3\sqrt{2})}^{14}i
\end{align*}
** $w$
$$\sin(\varphi_w) = \frac{\sqrt{3}}{\sqrt{4}} = \frac{\sqrt{3}}{2}
\to \varphi_w = \frac{2}{3} \pi$$

\begin{align*}
w^{11} &= 2^{11} \left( \cos \left(11 \cdot \frac{2}{3} \pi \right)
+ i \sin \left( 11 \cdot \frac{2}{3} \pi \right) \right)\\
&= 2^{11} \left( -\cos \frac{\pi}{3}
- i \sin \frac{\pi}{3} \right)\\
&= 2^{11} \left(- \frac{1}{2} - i \frac{\sqrt{3}}{2} \right)\\
&= 2^{10} \left(-1 - i \sqrt{3} \right)
\end{align*}
** Podstawiamy
\begin{align*}
\frac{ { (3 - 3i)}^{14} }
{ { (-1+i\sqrt{3}) }^{11} }
&= \frac{z^{14}}{w^{11}}\\
&=\frac{(3\sqrt{2})^{14} i }
{2^{10}(-1 -i\sqrt{3})}\\
&=\frac{ ((3\sqrt{2})^{14} i)(-1 + i\sqrt{3}) }
{2^{10}(-1 -i\sqrt{3})(-1 + i\sqrt{3})}\\
&=\frac{ ((3\sqrt{2})^{14} i)(-1 + i\sqrt{3}) }
{2^{10}(-2)}\\
&=\frac{ ((3\sqrt{2})^{14} i)(-1 + i\sqrt{3}) }
{-2^{11}}
\end{align*}
